theories/SpecNotations.v
@@ -35,24 +35,61 @@ Defined.
 
 (* Notation "D ⊢ E ⊠ D'" := (sE D E D') (at level 90). *)
 
+Definition c_true := c_unify E_tt E_tt t_unit.
+Definition c_and c c' := c_unify (E_match_tt c) (E_match_tt c') t_unit.
+
 Module RelNotations.
   Declare Custom Entry rel.
 
   Notation "<{ E }>" := E (E custom rel at level 99).
-  Notation "x" := x (in custom rel, x ident).
-  Notation "${ e }" := e (in custom rel, e constr).
+  Notation "x" := x (in custom rel at level 0, x constr).
+  Notation "( E )" := E (in custom rel, E custom rel at level 0).
+  Notation "${ e }" := e (in custom rel, e constr, only parsing).
+
+  Coercion t_var: sort >-> type.
 
   Notation "'I'" := t_unit (in custom rel at level 0).
   Notation "S ⊗ T" := (t_prod S T) (in custom rel at level 50, right associativity).
 
-  (* Notation "'λ' X , E" := *)
-  (*   (E_lam X E) *)
-  (*     (in custom rel at level 200, *)
-  (*         X constr at level 99, *)
-  (*         E custom rel at level 99, *)
-  (*         left associativity). *)
+  Definition X: var := 0.
+  Definition X1: var := 1.
+  Definition X2: var := 2.
 
-  Notation "( E , E' )" := (E_fanout E E') (in custom rel at level 30, right associativity).
+  Definition Y: var := 3.
+  Definition Z: var := 4.
+
+  Coercion V_var: var >-> elim.
 
   Coercion E_var: var >-> context.
+
+  Notation "⊤" := c_true (in custom rel).
+  Notation "⊥" := c_false (in custom rel).
+
+  Infix "∧" := c_and (in custom rel at level 30, right associativity).
+  Infix "∨" := c_or (in custom rel at level 30, right associativity).
+
+  Notation "!" := E_tt (in custom rel).
+  Infix "," := E_fanout (in custom rel at level 30, right associativity).
+
+  (* Notation "'del'" := E_del (in custom rel). *)
+  (* Notation "'dup'" := E_dup (in custom rel). *)
+  (* Notation "'unify'" := c_unify (in custom rel). *)
+
+  Notation "E '>>' c" := (c_unify E (E_match_tt c) t_unit) (in custom rel at level 30, right associativity).
+
+  (* Notation "'ε' . c" := (E_match_tt c) *)
+  (*                         (in custom rel at level 200, c custom rel at level 99, *)
+  (*                             left associativity). *)
+  (* Notation "'ε' X , Y . c" := (E_match_fanout X Y c) *)
+  (*                               (in custom rel at level 200, *)
+  (*                                   X constr at level 99, *)
+  (*                                   Y constr at level 99, *)
+  (*                                   c custom rel at level 99, *)
+  (*                                   left associativity). *)
+
+  (* Notation "'ε' X . c" := (E_epsilon X c) *)
+  (*                           (in custom rel at level 200, *)
+  (*                               X constr at level 99, *)
+  (*                               c custom rel at level 99, *)
+  (*                               left associativity). *)
 End RelNotations.
